Complete definition of SCL strategy part 1

Simulation_SCLFOL_Ordered_Resolution/Simulation.thy
@@ -550,25 +550,52 @@ proof -
     using \<open>ord_res.ground_factoring\<^sup>*\<^sup>* C C' \<and> (\<nexists>C''. ord_res.ground_factoring C' C'')\<close> by blast
 qed
 
-inductive scl_reso1_step1 :: "_ \<Rightarrow> ('f, 'v) scl_fol_sim_state \<Rightarrow> ('f, 'v) scl_fol_sim_state \<Rightarrow> bool" for N\<^sub>0 where
-  scl_reso1_step1I: "\<F> C \<prec>\<^sub>c \<F> D \<Longrightarrow> \<not> fBex (N\<^sub>0 |\<union>| fimage gcls_of_cls U) (\<lambda>D'. \<F> C \<prec>\<^sub>c \<F> D' \<and> \<F> D' \<prec>\<^sub>c \<F> D) \<Longrightarrow>
+term "propagate_lit L D Var"
+term "trail_propagate \<Gamma> L D' Var"
+
+find_theorems "?P (is_minimal_wrt _ _ _)"
+
+inductive scl_reso1 for N\<^sub>0 \<beta> where
+  scl_reso1I: "\<F> C \<prec>\<^sub>c \<F> D \<Longrightarrow> \<not> fBex (N\<^sub>0 |\<union>| fimage gcls_of_cls U) (\<lambda>D'. \<F> C \<prec>\<^sub>c \<F> D' \<and> \<F> D' \<prec>\<^sub>c \<F> D) \<Longrightarrow>
   ord_res.is_maximal_lit L D \<Longrightarrow>
   sorted_wrt (\<prec>\<^sub>l) Ks \<Longrightarrow> (\<forall>K \<in> set Ks. is_neg K \<and> K \<prec>\<^sub>l L \<and>
     \<not> trail_defined_lit \<Gamma> (lit_of_glit K) \<and>
     lit_occures_in_clss K N\<^sub>0) \<Longrightarrow>
-  \<Gamma>' = foldl trail_decide \<Gamma> (map lit_of_glit Ks) \<Longrightarrow>
-  scl_reso1_step1 N\<^sub>0 ((\<Gamma>, U, None), i, C, \<F>) ((\<Gamma>', U, None), i, D, \<F>)"
+  \<Gamma>\<^sub>1 = foldl trail_decide \<Gamma> (map lit_of_glit Ks) \<Longrightarrow>
+  S1 = ((\<Gamma>\<^sub>1, U, None :: ('f, 'v) closure option), i, D, \<F>) \<Longrightarrow>
+  \<F> D |\<in>| N\<^sub>0 \<Longrightarrow>
+  sfac D = sfac (\<F> D) \<Longrightarrow>
+  \<F> D = add_mset L D' \<Longrightarrow>
+  S2 =
+    (let
+      \<Gamma>\<^sub>2\<^sub>a = trail_decide \<Gamma>\<^sub>1 (lit_of_glit L);
+      \<Gamma>\<^sub>2\<^sub>b = trail_propagate \<Gamma>\<^sub>1 (lit_of_glit L) (cls_of_gcls D') Var;
+      E = (THE E. is_minimal_wrt (\<prec>\<^sub>c) E
+        {|C |\<in>| N\<^sub>0 |\<union>| fimage gcls_of_cls U. trail_false_cls \<Gamma>\<^sub>2\<^sub>b (cls_of_gcls C)|});
+      j\<^sub>0 = count D' L;
+      j = i + j\<^sub>0
+    in
+      (if is_pos L \<and> trail_false_cls \<Gamma>\<^sub>1 (cls_of_gcls D) then
+        (if (\<nexists>S'. scl_fol.conflict (cls_of_gcls |`| N\<^sub>0) (term_of_gterm \<beta>) (\<Gamma>\<^sub>2\<^sub>a, U, None) S') then
+          \<comment> \<open>2a\<close>
+          ((\<Gamma>\<^sub>2\<^sub>a, U, None :: ('f, 'v) closure option), j, D, \<F>(D := sfac D))
+        else
+          \<comment> \<open>2b\<close>
+          ((\<Gamma>\<^sub>2\<^sub>b, U, Some (cls_of_gcls E, Var)), j, D, \<F>(D := sfac D)))
+      else
+        \<comment> \<open>2c\<close>
+        S1)) \<Longrightarrow>
+  scl_reso1 N\<^sub>0 \<beta> ((\<Gamma>, U, None :: ('f, 'v) closure option), i, C, \<F>) S1 S2"
 
-lemma correctness_scl_reso1_step1:
+lemma correctness_scl_reso1:
   fixes N\<^sub>0 :: "'f gterm clause fset"
   assumes
-    \<beta>\<^sub>G_greatest: "is_greatest_in_set_wrt (\<prec>\<^sub>t) (atms_of_clss (fset N\<^sub>0)) \<beta>\<^sub>G" and
-    step: "scl_reso1_step1 N\<^sub>0 (S, i, C, \<F>) (S', i', C', \<F>')"
-  defines "\<beta> \<equiv> term_of_gterm \<beta>\<^sub>G"
-  shows "(scl_fol.decide (fimage cls_of_gcls N\<^sub>0) \<beta>)\<^sup>*\<^sup>* S S'"
+    \<beta>_greatest: "is_greatest_in_set_wrt (\<prec>\<^sub>t) (atms_of_clss (fset N\<^sub>0)) \<beta>" and
+    step: "scl_reso1 N\<^sub>0 \<beta> (S, i, C, \<F>) (S', i', C', \<F>') S2"
+  shows "(scl_fol.decide (fimage cls_of_gcls N\<^sub>0) (term_of_gterm \<beta>))\<^sup>*\<^sup>* S S'"
   using step
-proof (cases N\<^sub>0 "(S, i, C, \<F>)" "(S', i', C', \<F>')" rule: scl_reso1_step1.cases)
-  case hyps: (scl_reso1_step1I U L Ks \<Gamma> \<Gamma>')
+proof (cases N\<^sub>0 \<beta> "(S, i, C, \<F>)" "(S', i', C', \<F>')" rule: scl_reso1.cases)
+  case hyps: (scl_reso1I D U L Ks \<Gamma> \<Gamma>')
   then show ?thesis
   proof (induction Ks arbitrary: S \<Gamma>)
     case Nil
@@ -584,7 +611,8 @@ proof (cases N\<^sub>0 "(S, i, C, \<F>)" "(S', i', C', \<F>')" rule: scl_reso1_s
     from ball_K_Ks have "\<not> trail_defined_lit \<Gamma> (lit_of_glit K)" "lit_occures_in_clss K N\<^sub>0"
       by simp_all
 
-    from Cons have "(scl_fol.decide (fimage cls_of_gcls N\<^sub>0) \<beta>)\<^sup>*\<^sup>* (trail_decide \<Gamma> (lit_of_glit K), U, None) S'"
+    from Cons have "(scl_fol.decide (fimage cls_of_gcls N\<^sub>0) (term_of_gterm \<beta>))\<^sup>*\<^sup>*
+      (trail_decide \<Gamma> (lit_of_glit K), U, None) S'"
     proof (intro Cons.IH[OF refl] ballI)
       show "\<Gamma>' = foldl trail_decide (trail_decide \<Gamma> (lit_of_glit K)) (map lit_of_glit Ks)"
         by (simp add: \<open>\<Gamma>' = foldl trail_decide \<Gamma> (map lit_of_glit (K # Ks))\<close>)
@@ -616,7 +644,8 @@ proof (cases N\<^sub>0 "(S, i, C, \<F>)" "(S', i', C', \<F>')" rule: scl_reso1_s
         by simp
     qed
 
-    moreover have "scl_fol.decide (fimage cls_of_gcls N\<^sub>0) \<beta> (\<Gamma>, U, None) (trail_decide \<Gamma> (lit_of_glit K), U, None)"
+    moreover have "scl_fol.decide (fimage cls_of_gcls N\<^sub>0) (term_of_gterm \<beta>)
+      (\<Gamma>, U, None) (trail_decide \<Gamma> (lit_of_glit K), U, None)"
     proof (intro scl_fol.decideI[of _ _ Var, simplified])
       show "\<not> trail_defined_lit \<Gamma> (lit_of_glit K)"
         using \<open>\<not> trail_defined_lit \<Gamma> (lit_of_glit K)\<close> .
@@ -633,14 +662,15 @@ proof (cases N\<^sub>0 "(S, i, C, \<F>)" "(S', i', C', \<F>')" rule: scl_reso1_s
         using \<open>lit_occures_in_clss K N\<^sub>0\<close>
         unfolding lit_occures_in_clss_def atms_of_clss_def
         by (metis Union_iff atms_of_def image_eqI)
-      thus "ground (atm_of (lit_of_glit K)) \<and> ground \<beta> \<and>
-        gterm_of_term (atm_of (lit_of_glit K)) \<prec>\<^sub>t gterm_of_term \<beta> \<or> atm_of (lit_of_glit K) = \<beta>"
-        using \<beta>\<^sub>G_greatest
-        by (auto simp add: atm_of_lit_of_glit_conv \<beta>_def is_greatest_in_set_wrt_iff)
+      thus "ground (atm_of (lit_of_glit K)) \<and> ground (term_of_gterm \<beta>) \<and>
+        gterm_of_term (atm_of (lit_of_glit K)) \<prec>\<^sub>t gterm_of_term (term_of_gterm \<beta>) \<or>
+        atm_of (lit_of_glit K) = (term_of_gterm \<beta>)"
+        using \<beta>_greatest
+        by (auto simp add: atm_of_lit_of_glit_conv is_greatest_in_set_wrt_iff)
     qed
 
     ultimately show ?case
-      unfolding \<open>S = (\<Gamma>, U, None)\<close> \<open>S' = (\<Gamma>', U, None)\<close>
+      unfolding \<open>S = (\<Gamma>, U, None)\<close> \<open>(S', i', C', \<F>') = ((\<Gamma>', U, None), i, D, \<F>)\<close>
         \<open>\<Gamma>' = foldl trail_decide \<Gamma> (map lit_of_glit (K # Ks))\<close>
       by simp
   qed
